src/program_proof/rsm/spaxos_ghost.v
@@ -1,0 +1,98 @@
+(**
+ * Ghost state definitions, type class instances, and rules.
+ *)
+From Perennial.program_proof Require Import spaxos_top.
+From Perennial.base_logic Require Import ghost_map mono_nat.
+From iris.algebra Require Import mono_nat mono_list gmap_view gset.
+
+Inductive consensus : Set :=
+| Chosen (v : string)
+| Free.
+
+Class spaxos_ghostG (Σ : gFunctors).
+
+Record spaxos_names := {}.
+
+Section consensus.
+  Context `{!spaxos_ghostG Σ}.
+  (* TODO: remove this once we have real defintions for resources. *)
+  Implicit Type (γ : spaxos_names).
+
+  (* Definitions. *)
+  Definition is_chosen γ (v : string) : iProp Σ.
+  Admitted.
+
+  Definition own_free γ : iProp Σ.
+  Admitted.
+
+  (* Type class instances. *)
+  Instance is_chosen_persistent γ :
+    Persistent (∀ v, is_chosen γ v).
+  Admitted.
+  
+  (* Rules. *)
+  Lemma consensus_update {γ} v :
+    own_free γ ==∗
+    is_chosen γ v.
+  Admitted.
+
+  Lemma consensus_agree {γ} v1 v2 :
+    is_chosen γ v1 -∗
+    is_chosen γ v2 -∗
+    ⌜v1 = v2⌝.
+  Admitted.
+End consensus.
+
+Section proposal.
+  Context `{!spaxos_ghostG Σ}.
+  (* TODO: remove this once we have real defintions for resources. *)
+  Implicit Type (γ : spaxos_names).
+
+  (* Definitions. *)
+  Definition is_proposal γ (n : nat) (v : string) : iProp Σ.
+  Admitted.
+
+  Definition own_proposals γ (ps : gmap nat string) : iProp Σ.
+  Admitted.
+  
+  (* Type class instances. *)
+  Instance is_proposal_persistent γ :
+    Persistent (∀ n v, is_proposal γ n v).
+  Admitted.
+
+  (* Rules. *)
+  Lemma proposals_insert {γ} ps n v :
+    ps !! n = None ->
+    own_proposals γ ps ==∗
+    own_proposals γ (<[n := v]> ps) ∗ is_proposal γ n v.
+  Admitted.
+End proposal.
+
+Section ballot.
+  Context `{!spaxos_ghostG Σ}.
+  (* TODO: remove this once we have real defintions for resources. *)
+  Implicit Type (γ : spaxos_names).
+
+  (* Definitions. *)
+  Definition own_ballot γ (x : nat) (b : ballot) : iProp Σ.
+  Admitted.
+
+  Definition is_ballot_lb γ (x : nat) (b : ballot) : iProp Σ.
+  Admitted.
+
+  Definition own_ballots γ (bs : gmap nat ballot) : iProp Σ.
+  Admitted.
+
+  (* Type class instances. *)
+  Instance is_ballot_lb_persistent γ :
+    Persistent (∀ x b, is_ballot_lb γ x b).
+  Admitted.
+
+  (* Rules. *)
+  Lemma ballot_update {γ} bs x b b' :
+    prefix b b' ->
+    own_ballot γ x b -∗
+    own_ballots γ bs ==∗
+    own_ballot γ x b' ∗ own_ballots γ (<[x := b']> bs).
+  Admitted.
+End ballot.
