src/program_proof/rsm/spaxos_prelude.v
@@ -1,0 +1,3 @@
+From Perennial.program_proof.rsm Require Export
+  spaxos_top spaxos_ghost spaxos_inv.
+From Goose.github_com.mit_pdos.rsm Require Export spaxos.
