src/program_proof/rsm/spaxos_top.v
@@ -1,0 +1,7 @@
+(**
+ * Common definitions used by every part of this project. Minimize this file.
+ *)
+From Perennial.program_proof Require Export grove_prelude.
+
+Definition proposals := gmap nat string.
+Definition ballot := list bool.
