src/program_proof/rsm/goose.sh
@@ -1,0 +1,4 @@
+#!/bin/bash
+
+cd ../../../
+./etc/update-goose.py --compile --goose ../goose/ --rsm ../rsm/
